WIP

src/Label.v
@@ -77,41 +77,41 @@ Definition label_opt_eqb s1 s2 : bool :=
   | right _ => false
   end.
 
-Definition label_opt_eqb_reflexive so :
+Lemma label_opt_eqb_reflexive so :
   label_opt_eqb so so = true.
 Proof.
   unfold label_opt_eqb; destruct label_opt_dec; easy.
-Defined.
+Qed.
 
-Definition label_opt_eqb_symmetric so1 so2 :
+Lemma label_opt_eqb_symmetric so1 so2 :
   label_opt_eqb so1 so2 = label_opt_eqb so2 so1.
 Proof.
   unfold label_opt_eqb.
   destruct (label_opt_dec so1 so2), (label_opt_dec so2 so1);
     try congruence; easy.
-Defined.
+Qed.
 
-Definition label_opt_eqb_transitive so1 so2 so3 :
+Lemma label_opt_eqb_transitive so1 so2 so3 :
   label_opt_eqb so1 so2 = true ->
   label_opt_eqb so2 so3 = label_opt_eqb so1 so3.
 Proof.
   intros H; unfold label_opt_eqb in H.
   destruct (label_opt_dec so1 so2) as [Heq|]; try easy.
   rewrite Heq; easy.
-Defined.
+Qed.
 
 Definition is_less_than_label_opt so1 so2 :=
   match so1, so2 with
   | None, None => false
-  | Some s1, None => false
-  | None, Some s2 => true
+  | Some s1, None => true
+  | None, Some s2 => false
   | Some s1, Some s2 => is_less_than_label s1 s2
   end.
 
 Definition less_than_label_opt so1 so2 :=
   if is_less_than_label_opt so1 so2 then sUnit else sEmpty.
 
-Definition is_less_than_ascii_asymmetric a1 a2 :
+Lemma is_less_than_ascii_asymmetric a1 a2 :
   is_less_than_ascii a1 a2 = true ->
   is_less_than_ascii a2 a1 = false.
 Proof.
@@ -125,9 +125,9 @@ Proof.
             destruct b3, b11; try easy;
               destruct b2, b10; try easy;
                 destruct b1, b9; easy.
-Defined.
+Qed.
 
-Definition is_less_than_ascii_total a1 a2 :
+Lemma is_less_than_ascii_total a1 a2 :
   is_less_than_ascii a1 a2 = false ->
   is_less_than_ascii a2 a1 = false ->
   a1 = a2.
@@ -142,9 +142,9 @@ Proof.
             destruct b3, b11; try easy;
               destruct b2, b10; try easy;
                 destruct b1, b9; easy.
-Defined.
+Qed.
 
-Definition is_less_than_ascii_transitive a1 a2 a3 :
+Lemma is_less_than_ascii_transitive a1 a2 a3 :
   is_less_than_ascii a1 a2 = true ->
   is_less_than_ascii a2 a3 = true ->
   is_less_than_ascii a1 a3 = true.
@@ -160,9 +160,9 @@ Proof.
             destruct b3, b11, b19; try easy;
               destruct b2, b10, b18; try easy;
                 destruct b1, b9, b17; easy.
-Defined.
+Qed.
 
-Definition is_less_than_label_asymmetric s1 s2 :
+Lemma is_less_than_label_asymmetric s1 s2 :
   is_less_than_label s1 s2 = true ->
   is_less_than_label s2 s1 = false.
 Proof.
@@ -177,9 +177,9 @@ Proof.
           apply is_less_than_ascii_asymmetric; easy).
     easy.
   - apply IHs1.
-Defined.
+Qed.
 
-Definition is_less_than_label_total s1 s2 :
+Lemma is_less_than_label_total s1 s2 :
   is_less_than_label s1 s2 = false ->
   is_less_than_label s2 s1 = false ->
   s1 = s2.
@@ -194,9 +194,9 @@ Proof.
     by (apply is_less_than_ascii_total; easy).
   intros; replace s2 with s1 by (apply IHs1; easy).
   easy.
-Defined.
+Qed.
 
-Definition is_less_than_label_transitive s1 s2 s3 :
+Lemma is_less_than_label_transitive s1 s2 s3 :
   is_less_than_label s1 s2 = true ->
   is_less_than_label s2 s3 = true ->
   is_less_than_label s1 s3 = true.
@@ -224,17 +224,17 @@ Proof.
       [|destruct (is_less_than_ascii a3 a2) eqn:Heq4];
       try easy.
     apply IHs1.
-Defined.
+Qed.
 
-Definition is_less_than_label_opt_asymmetric so1 so2 :
+Lemma is_less_than_label_opt_asymmetric so1 so2 :
   is_less_than_label_opt so1 so2 = true ->
   is_less_than_label_opt so2 so1 = false.
 Proof.
   destruct so1, so2; cbn; try easy.
   apply is_less_than_label_asymmetric.
-Defined.
+Qed.
 
-Definition is_less_than_label_opt_total so1 so2 :
+Lemma is_less_than_label_opt_total so1 so2 :
   is_less_than_label_opt so1 so2 = false ->
   is_less_than_label_opt so2 so1 = false ->
   so1 = so2.
@@ -244,24 +244,21 @@ Proof.
   replace s1 with s2
     by (apply is_less_than_label_total; easy).
   easy.
-Defined.
+Qed.
 
-Definition is_less_than_label_opt_transitive so1 so2 so3 :
+Lemma is_less_than_label_opt_transitive so1 so2 so3 :
   is_less_than_label_opt so1 so2 = true ->
   is_less_than_label_opt so2 so3 = true ->
   is_less_than_label_opt so1 so3 = true.
 Proof.
   destruct so1, so2, so3; cbn; try easy.
   apply is_less_than_label_transitive.
-Defined.
+Qed.
 
-Definition is_less_than_label_opt_irreflexive so1 so2 :
-  is_less_than_label_opt so1 so2 = true ->
-  label_opt_eqb so1 so2 = false.
+Lemma is_less_than_label_opt_irreflexive so :
+  is_less_than_label_opt so so = false.
 Proof.
-  intros H1; unfold label_opt_eqb.
-  apply is_less_than_label_opt_asymmetric in H1 as H2.
-  destruct (label_opt_dec so1 so2) as [Heq|]; try easy.
-  rewrite Heq in H1, H2.
-  rewrite H1 in H2; easy.
-Defined.
+  destruct (is_less_than_label_opt so so) eqn:Heq1; try easy.
+  apply is_less_than_label_opt_asymmetric in Heq1 as Heq2.
+  rewrite Heq2 in Heq1; easy.
+Qed.
