src/Renaming.v
@@ -1,5 +1,5 @@
 Require Import Label PeanoNat Psatz Compare_dec StrictProp.
-Require Import Var.
+Require Import Var VarEquations.
 
 Inductive raw_renaming :=
   | raw_renaming_id : raw_renaming
@@ -14,17 +14,17 @@ Fixpoint is_interesting_raw_renaming_extension v r vo :=
       (unshift_var v' v) r (unshift_var_opt vo' vo)
   end.
 
-Definition is_ordered_raw_renaming_var r v :=
+Definition is_ordered_raw_renaming_var v r :=
   match r with
   | raw_renaming_id => true
-  | raw_renaming_extend v' _ _ => is_less_equal_vars v' v
+  | raw_renaming_extend v' _ _ => is_less_equal_vars v v'
   end.
 
 Fixpoint is_normalized_raw_renaming r :=
   match r with
   | raw_renaming_id => true
   | raw_renaming_extend v r vo =>
-    andb (is_ordered_raw_renaming_var r v)
+    andb (is_ordered_raw_renaming_var v r)
          (andb (is_interesting_raw_renaming_extension v r vo)
                (is_normalized_raw_renaming r))
   end.
@@ -32,7 +32,7 @@ Fixpoint is_normalized_raw_renaming r :=
 Definition normalized_raw_renaming r :=
   if is_normalized_raw_renaming r then sUnit else sEmpty.
 
-Definition normalized_raw_renaming_from_extend {v r vo} :
+Lemma normalized_raw_renaming_from_extend {v r vo} :
   normalized_raw_renaming (raw_renaming_extend v r vo) ->
   normalized_raw_renaming r.
 Proof.
@@ -69,7 +69,7 @@ Fixpoint raw_renaming_extend_boring v r vo :=
     end
   end.
 
-Definition is_interesting_raw_renaming_extend_boring_none v r vo :
+Lemma is_interesting_raw_renaming_extend_boring_none v r vo :
   raw_renaming_extend_boring v r vo = None ->
   is_interesting_raw_renaming_extension v r vo = true.
 Proof.
@@ -81,60 +81,141 @@ Proof.
     destruct (raw_renaming_extend_boring
                 (unshift_var v' v) r (unshift_var_opt vo' vo));
       easy.
-Defined.
+Qed.
 
-Definition v_label_opt_shift v1 v2 :
-  v_label_opt (shift_var v1 v2) = v_label_opt v2.
+Lemma is_normalized_raw_renaming_extend_boring_none
+      r v1 v2 vo1 vo2 :
+  is_normalized_raw_renaming (raw_renaming_extend v2 r vo2)
+  = true ->
+  raw_renaming_extend_boring
+    v1 (raw_renaming_extend v2 r vo2) vo1 = None ->
+  is_less_equal_vars v1 v2 = true ->
+  is_normalized_raw_renaming
+    (raw_renaming_extend v1 (raw_renaming_extend v2 r vo2) vo1)
+    = true.
 Proof.
-  destruct v1 as [n1|], v2 as [n2|]; cbn; try easy.
-  unfold shift_name.
-  destruct (label_dec (n_label n1) (n_label n2)); try easy.
-  destruct (le_gt_dec (n_index n1) (n_index n2)); easy.
-Defined.
-(*
-Definition is_ordered_vars_shift v1 v2 v3 :
-  is_ordered_vars v3 v1 = true ->
-  is_ordered_vars
-    (shift_var (unshift_var v1 v2) v3) (shift_var v2 v1) = true.
+  intros Heq1 Heq2 Heq3; cbn in *.
+  rewrite Heq3, Heq1.
+  rewrite is_interesting_raw_renaming_extend_boring_none; try easy.
+  destruct (raw_renaming_extend_boring (unshift_var v2 v1) r
+             (unshift_var_opt vo2 vo1)); easy.
+Qed.
+
+(* TODO move to VarEquations.v *)
+Lemma var_opt_var_eqb_some_true v1 v2 :
+  var_opt_var_eqb (Some v1) v2 = true <-> v1 = v2.
 Proof.
-  unfold is_ordered_vars.
-  rewrite !v_label_opt_shift.
-  destruct
-    (is_less_than_label_opt (v_label_opt v3) (v_label_opt v1));
-    try easy.
-  unfold label_opt_eqb.
-  destruct (label_opt_dec (v_label_opt v3) (v_label_opt v1));
-    try easy.
-  rewrite !Bool.orb_false_l, !Bool.andb_true_l; intros Heq2.
-  destruct v1 as [n1|l1], v2 as [n2|l2], v3 as [n3|l3]; cbn in *;
-    try easy.
-  - apply leb_correct; apply leb_complete in Heq2.
-    assert (n_label n3 = n_label n1) by congruence.
-    unfold shift_name, unshift_name.
-    destruct (label_dec (n_label n1) (n_label n2));
-      destruct (label_dec (n_label n2) (n_label n1)); cbn;
-        try congruence.
-    destruct (le_gt_dec (n_index n2) (n_index n1)).
-    + destruct (label_dec (n_label n2) (n_label n3));
-        destruct (le_gt_dec (n_index n2) (n_index n3)); cbn; lia.
-    + destruct label_dec; try easy.
-      destruct le_gt_dec; try easy.
-      cbn in *.
-      destruct (n_index n2); cbn in *; try lia.
-      assert (i < S (n_index n3)) by lia.
-      destruct n1, n2, n3; cbn in *; subst.
-      destruct n_index1.
-      * admit.
-      * 
-*)
-(*
-Definition is_ordered_raw_renaming_extend_boring_shift
+  unfold var_opt_var_eqb.
+  destruct (var_opt_var_dec (Some v1) v2).
+  - replace v1 with v2 by congruence; easy.
+  - split; intro; congruence.
+Qed.
+
+Lemma var_opt_var_eqb_some_false v1 v2 :
+  var_opt_var_eqb (Some v1) v2 = false <-> v1 <> v2.
+Proof.
+  unfold var_opt_var_eqb.
+  destruct (var_opt_var_dec (Some v1) v2).
+  - replace v1 with v2 by congruence; easy.
+  - split; intro; congruence.
+Qed.
+
+Lemma succ_var_injective v1 v2 :
+  v1 <> v2 ->
+  succ_var v1 <> succ_var v2.
+Proof.
+  intros Hneq Heq; apply Hneq.
+  replace v1 with (pred_var (succ_var v1))
+    by (reduce_vars; easy).
+  replace v2 with (pred_var (succ_var v2))
+    by (reduce_vars; easy).
+  congruence.
+Qed.
+
+Lemma mk_var_label_injective v1 v2 :
+  v_label_opt v1 <> v_label_opt v2 ->
+  v1 <> v2.
+Proof.
+  intros Hneq Heq; apply Hneq.
+  rewrite Heq; easy.
+Qed.
+
+Lemma is_interesting_raw_renaming_extend_boring_shift_ind
+      r1 :
+  forall r2 v1 v2 v3 v4 vo1 vo2 vo3 vo4,
+  is_interesting_raw_renaming_extension v1 r1 vo1 = true ->
+  v3 = unshift_var v1 v2 ->
+  vo3 = unshift_var_opt vo1 vo2 ->
+  raw_renaming_extend_boring v3 r1 vo3 = Some r2 ->
+  v4 = shift_var v2 v1 ->
+  vo4 = shift_var_opt vo2 vo1 ->
+  is_interesting_raw_renaming_extension v4 r2 vo4 = true.
+Proof.
+  induction r1 as [|v5 r1 IHr1 vo5]; cbn;
+    intros * Heq1 -> -> Heq2 -> ->.
+  - destruct
+      (var_opt_var_eqb (unshift_var_opt vo1 vo2)
+                       (unshift_var v1 v2)) eqn:Heq3; try easy.
+    replace r2 with raw_renaming_id by congruence; cbn.
+    rewrite Bool.negb_true_iff in *.
+    destruct vo1 as [v3|], vo2 as [v4|]; cbn in *; try easy.
+    rewrite var_opt_var_eqb_some_false, var_opt_var_eqb_some_true
+      in *.
+    generalize Heq3.
+    case_vars v1 v2; case_vars v3 v4; try easy;
+      intros; subst; reduce_vars;
+        autorewrite with reduce_vars_beta in *;
+        try solve [rewrite red_var_neq
+                    by solve_v_label_opt_equation;
+                   reduce_vars_beta; lia];
+        try solve [apply mk_var_label_injective;
+                   solve_v_label_opt_equation];
+        solve [apply succ_var_injective; easy].
+  - destruct
+      (raw_renaming_extend_boring
+         (unshift_var v5 (unshift_var v1 v2)) r1
+         (unshift_var_opt vo5 (unshift_var_opt vo1 vo2)))
+      as [r3|] eqn:Heq3; try easy.
+    replace r2 with
+        (raw_renaming_extend
+              (shift_var (unshift_var v1 v2) v5) r3
+              (shift_var_opt (unshift_var_opt vo1 vo2) vo5))
+      by congruence; cbn.
+    eapply IHr1
+      with (v1 := unshift_var v5 v1)
+           (vo1 := unshift_var_opt vo5 vo1)
+           (v2 := unshift_var (shift_var v1 v5) v2)
+           (vo2 := unshift_var_opt (shift_var_opt vo1 vo5) vo2)
+           (v3 := unshift_var v5 (unshift_var v1 v2))
+           (vo3 := unshift_var_opt vo5 (unshift_var_opt vo1 vo2));
+      try easy.
+    + rewrite transpose_pops_reverse_right; easy.
+    + rewrite transpose_pushes_reverse_left; easy.
+    + rewrite transpose_pops_reverse_middle; easy.
+    + rewrite transpose_pushes_reverse_middle; easy.
+Qed.
+
+Lemma is_interesting_raw_renaming_extend_boring_shift
+      {r1 r2 v1 v2 vo1 vo2} :
+  is_interesting_raw_renaming_extension v1 r1 vo1 = true ->
+  raw_renaming_extend_boring
+    (unshift_var v1 v2) r1 (unshift_var_opt vo1 vo2) = Some r2 ->
+  is_interesting_raw_renaming_extension
+    (shift_var v2 v1) r2 (shift_var_opt vo2 vo1) = true.
+Proof.
+  intros Heq1 Heq2.
+  apply (is_interesting_raw_renaming_extend_boring_shift_ind
+           r1 r2 v1 v2 _ _ vo1 vo2 _ _ Heq1 eq_refl eq_refl Heq2
+           eq_refl eq_refl).
+Qed.
+
+Lemma is_ordered_raw_renaming_extend_boring_shift
            r1 r2 v1 v2 vo1 vo2 :
-  is_ordered_raw_renaming_var r1 v1 = true ->
+  is_ordered_raw_renaming_var v1 r1 = true ->
   raw_renaming_extend_boring
     (unshift_var v1 v2) r1 (unshift_var_opt vo1 vo2)
   = Some r2 ->
-  is_ordered_raw_renaming_var r2 (shift_var v2 v1) = true.
+  is_ordered_raw_renaming_var (shift_var v2 v1) r2 = true.
 Proof.
   generalize dependent v1.
   generalize dependent v2.
@@ -155,37 +236,15 @@ Proof.
               (shift_var (unshift_var v1 v2) v3) r
               (shift_var_opt (unshift_var_opt vo1 vo2) vo3))
       by congruence; cbn.
-    
-
-Defined
-*)
-
-Definition is_ordered_raw_renaming_transitive r v1 v2 :
-  is_ordered_raw_renaming_var r v1 = true ->
-  is_less_equal_vars v1 v2 = true ->
-  is_ordered_raw_renaming_var r v2 = true.
-Proof.
-  intros Heq1 Heq2.
-  destruct r; cbn in *; try easy.
-  apply is_less_equal_vars_transitive with (v2 := v1); easy.
+    generalize Heq1.
+    case_vars v1 v2; case_vars v1 v3; try easy.
+    + case_vars (pred_var v2) v3; easy.
+    + case_vars (pred_var v2) v1; easy.
 Qed.
 
-Definition is_ordered_unshift r v1 v2 :
-  is_ordered_raw_renaming_var r v1 = true ->
-  is_ordered_vars v1 v2 = true ->
-  is_ordered_raw_renaming_var r (unshift_var v1 v2) = true.
-Proof.
-  intros Heq1 Heq2.
-  destruct v1 as [n1|l1], v2 as [n2|l2]; cbn; try easy.
-  - unfold unshift_name.
-    destruct label_dec.
-    + admit.
-    + 
-
-Definition is_normalized_raw_renaming_extend_boring_some
+Lemma is_normalized_raw_renaming_extend_boring_some
            v r vo r' :
   is_normalized_raw_renaming r = true ->
-  is_ordered_raw_renaming_var r v = true ->
   raw_renaming_extend_boring v r vo = Some r' ->
   is_normalized_raw_renaming r' = true.
 Proof.
@@ -193,11 +252,11 @@ Proof.
   generalize dependent vo.
   generalize dependent r'.
   induction r as [|v' r IHr vo']; cbn;
-    intros r' vo v Heq1 Heq2 Heq3.
+    intros r' vo v Heq1 Heq2.
   - destruct (var_opt_var_eqb vo v); try easy.
     replace r' with (raw_renaming_id) by congruence.
     easy.
-  - destruct (is_ordered_raw_renaming_var r v')
+  - destruct (is_ordered_raw_renaming_var v' r)
       eqn:Heq4; try easy.
     destruct (is_interesting_raw_renaming_extension v' r vo')
       eqn:Heq5; try easy.
@@ -210,30 +269,26 @@ Proof.
       with (raw_renaming_extend (shift_var v v')
               r'' (shift_var_opt vo vo'))
       by congruence; cbn.
-    replace (is_normalized_raw_renaming r'') with true.
-    admit.
-symmetry. apply IHr with (v := unshift_var v' v)
-           (vo := unshift_var_opt vo' vo). 
-easy.
-
-
-      by (symmetry; apply IHr with (v := unshift_var v' v)
-           (vo := unshift_var_opt vo' vo); easy).
-    
-
-    + eapply IHr.
-
-    apply IHr in Heq2.
-
-Defined.
-
-
+    replace (is_normalized_raw_renaming r'') with true
+      by (symmetry;
+          apply IHr with (v := unshift_var v' v)
+            (vo := unshift_var_opt vo' vo); easy).
+    rewrite is_ordered_raw_renaming_extend_boring_shift
+      with (r1 := r) (vo1 := vo') (vo2 := vo) by easy.
+    rewrite (is_interesting_raw_renaming_extend_boring_shift
+               Heq5 Heq7).
+    easy.
+Qed.
 
 Fixpoint normalized_raw_renaming_extend v r vo :=
   match r with
-  | raw_renaming_id => raw_renaming_extend v r vo
+  | raw_renaming_id =>
+    match raw_renaming_extend_boring v r vo with
+    | Some r => r
+    | None => raw_renaming_extend v r vo
+    end
   | raw_renaming_extend v' r' vo' =>
-    if is_ordered_vars v' v then
+    if is_less_equal_vars v v' then
       match raw_renaming_extend_boring v r vo with
       | Some r => r
       | None => raw_renaming_extend v r vo
@@ -245,6 +300,38 @@ Fixpoint normalized_raw_renaming_extend v r vo :=
            (unshift_var v' v) r' (unshift_var_opt vo' vo))
         (shift_var_opt vo vo')
   end.
+
+Lemma normalized_raw_renaming_extend_normalized v r vo :
+  normalized_raw_renaming r ->
+  normalized_raw_renaming
+    (normalized_raw_renaming_extend v r vo).
+Proof.
+  unfold normalized_raw_renaming.
+  destruct (is_normalized_raw_renaming r) eqn:Heq1;
+    try easy; intros _.
+  generalize dependent v.
+  generalize dependent vo.
+  induction r as [|v' r IHr vo']; intros vo v.
+  - cbn; destruct var_opt_var_eqb eqn:Heq2; cbn; try easy.
+    rewrite Heq2; easy.
+  - unfold normalized_raw_renaming_extend.
+    destruct (is_less_equal_vars v v') eqn:Heq6.
+    + destruct (raw_renaming_extend_boring
+                  v (raw_renaming_extend v' r vo') vo)
+               eqn:Heq7.
+      * rewrite is_normalized_raw_renaming_extend_boring_some
+          with (r := raw_renaming_extend v' r vo')
+               (v := v) (vo := vo); easy.
+      * rewrite is_normalized_raw_renaming_extend_boring_none
+          with (r := r) (v1 := v) (v2 := v')
+               (vo1 := vo) (vo2 := vo'); try easy.
+    + specialize
+        (IHr eq_refl (unshift_var_opt vo' vo) (unshift_var v' v)).
+      destruct (is_normalized_raw_renaming
+                  (normalized_raw_renaming_extend
+                     (unshift_var v' v) r (unshift_var_opt vo' vo)))
+               eqn:Heq7; try easy.
+Qed.
 
 Definition var_opt_geb vo1 vo2 :=
   match vo1, vo2 with
@@ -258,7 +345,7 @@ Definition var_opt_geb vo1 vo2 :=
 Definition var_nonzero vo :=
     negb (var_opt_eqb vo zero_var_opt) = true.
 
-Definition var_nonzero_shift vo1 vo2 :
+Lemma var_nonzero_shift vo1 vo2 :
   var_nonzero vo2 ->
   var_nonzero (shift_var_opt vo1 vo2).
 Proof.
@@ -266,9 +353,9 @@ Proof.
     cbn; try easy.
   unfold shift_level.
   destruct (le_gt_dec (S l1) (S l2)); easy.
-Defined.
+Qed.
 
-Definition var_nonzero_unshift vo1 vo2 vo3 :
+Lemma var_nonzero_unshift vo1 vo2 vo3 :
   (var_nonzero vo1 -> var_nonzero vo2) ->
   var_nonzero (unshift_var_opt vo3 vo1) ->
   var_nonzero (unshift_var_opt vo3 vo2).
@@ -276,7 +363,7 @@ Proof.
   destruct vo1 as [[n1|[|l1]]|], vo2 as [[n2|[|l2]]|],
     vo3 as [[n3|[|l3]]|]; cbn; try easy.
 
-Definition is_normalized_raw_renaming_entry_greater so vo1 vo2 r :
+Lemma is_normalized_raw_renaming_entry_greater so vo1 vo2 r :
   (var_nonzero vo1 -> var_nonzero vo2) ->
   is_normalized_raw_renaming_entry so vo1 r = true ->
   is_normalized_raw_renaming_entry so vo2 r = true.
@@ -289,7 +376,7 @@ Proof.
   apply IHr.
 
 
-Definition var_nonzero_unshift vo1 vo2 :
+Lemma var_nonzero_unshift vo1 vo2 :
   var_nonzero (unshift_var_opt vo1 vo2) ->
   var_nonzero vo1 \/ var_nonzero vo2
 Proof.
@@ -299,7 +386,7 @@ Proof.
 
   split.
 
-Definition is_normalized_raw_renaming_entry_unshift_shift
+Lemma is_normalized_raw_renaming_entry_unshift_shift
            so vo1 vo2 vo3 r :
   is_normalized_raw_renaming_entry so
     (unshift_var_opt vo3 vo1) r = true ->
@@ -311,7 +398,7 @@ Proof.
   - destruct (label_opt_eqb so so2); try easy.
     
 
-Definition raw_renaming_cons_null_entry_preserves_entries
+Lemma raw_renaming_cons_null_entry_preserves_entries
            so1 vo1 r1 r2 so2 vo2 :
   is_normalized_raw_renaming_entry so1 vo1 r1 = true ->
   raw_renaming_cons_null_entry so2 vo2 r1 = Some r2 ->
@@ -333,7 +420,7 @@ Proof.
     destruct (label_opt_eqb so1 so3); try easy.
     apply IHr1 with (vo2 := unshift_var_opt vo3 vo2); try easy.
 
-Definition raw_renaming_cons_null_entry_some so vo r r' :
+Lemma raw_renaming_cons_null_entry_some so vo r r' :
   normalized_raw_renaming r ->
   raw_renaming_cons_null_entry so vo r = Some r' ->
   normalized_raw_renaming r'.
@@ -351,19 +438,19 @@ Definition raw_renaming_cons_null_entry_some so vo r r' :
       try easy.
     apply IHr in Heq.
     
-Defined.
+Qed.
 
-Definition raw_renaming_cons_null_entry_none so vo r r' :
+Lemma raw_renaming_cons_null_entry_none so vo r r' :
   raw_renaming_cons_null_entry so vo r = None ->
   is_normalized_raw_renaming_entry so vo r.
-Defined.
+Qed.
 
-Definition normalized_raw_renaming_cons_normalized
+Lemma normalized_raw_renaming_cons_normalized
            {so vo r} :
   normalized_raw_renaming r ->
   normalized_raw_renaming
     (normalized_raw_renaming_cons so vo r).
-Proof. destruct vo as [[|[]]|], r; easy. Defined.
+Proof. destruct vo as [[|[]]|], r; easy. Qed.
 
 Definition closing_cons0 vo r :=
   mkclosing
@@ -403,7 +490,7 @@ Fixpoint raw_closing_cons l vo r :=
          (raw_closing_tl r))
   end.
 
-Definition raw_closing_cons_normalized {l vo r} :
+Lemma raw_closing_cons_normalized {l vo r} :
   normalized_pushes r ->
   normalized_pushes (raw_closing_cons l vo r).
 Proof.
@@ -414,7 +501,7 @@ Proof.
   apply IHl.
   destruct r as [|vo' r]; try easy.
   apply normalized_pushes_from_cons in Hnorm; easy.
-Defined.
+Qed.
 
 Definition closing_cons l vo r :=
   mkclosing
@@ -480,14 +567,14 @@ Definition closing_rhs_exchange0 l r :=
 Definition closing_rhs_close0 n r :=
   closing_rhs_cons0 (Some (free n)) r.
 
-Definition closing_rhs_cons0_normalized {vo r} :
+Lemma closing_rhs_cons0_normalized {vo r} :
   normalized_closing_rhs r ->
   normalized_closing_rhs (closing_rhs_cons0 vo r).
 Proof.
   destruct r as [? []]; cbn;
     apply normalized_pushes_cons_normalized;
     easy.
-Defined.
+Qed.
 
 Fixpoint transpose_push_raw_closing vo r {struct r} :=
   match r with
@@ -499,7 +586,7 @@ Fixpoint transpose_push_raw_closing vo r {struct r} :=
               (unshift_var_var_opt zero_var vo) r)
   end.
 
-Definition transpose_push_raw_closing_normalized {vo r} :
+Lemma transpose_push_raw_closing_normalized {vo r} :
   normalized_pushes r ->
   normalized_closing_rhs
     (transpose_push_raw_closing vo r).
@@ -510,7 +597,7 @@ Proof.
   destruct (var_opt_eqb vo zero_var_opt); try easy.
   apply closing_rhs_cons0_normalized.
   apply IHr; easy.
-Defined.
+Qed.
 
 Fixpoint compose_raw_closing r1 r2 :=
   match r1 with
@@ -522,7 +609,7 @@ Fixpoint compose_raw_closing r1 r2 :=
       (compose_raw_closing r1 (rhs_raw_closing rhs))
   end.
 
-Definition compose_raw_closing_normalized {r1 r2} :
+Lemma compose_raw_closing_normalized {r1 r2} :
   normalized_pushes r1 ->
   normalized_pushes r2 ->
   normalized_pushes (compose_raw_closing r1 r2).
@@ -533,7 +620,7 @@ Proof.
   apply normalized_pushes_cons_normalized.
   apply IHr1; try easy.
   apply transpose_push_raw_closing_normalized; easy.
-Defined.
+Qed.
 
 Definition compose_closing r1 r2 :=
   mkclosing
